Before getting rid of unify and trying to speed up fix_dom.

co_kind.v
@@ -3,7 +3,9 @@ Require Import LibTactics.
 Require Import Program.Wf.
 Require Import Arith.
 
-Require Import coercion type tactics ty_kind subst.
+Require Import coercion type tactics ty_kind subst var.
+
+Set Implicit Arguments.
 
 Reserved Notation "Si |-co g ~: t1 ~~ t2" (at level 67, t1 at next level).
 Inductive co_kind : ctxt -> coercion -> type -> type -> Prop :=
@@ -20,10 +22,14 @@ Inductive co_kind : ctxt -> coercion -> type -> type -> Prop :=
 | CKArrow : forall Si g1 g2 t1 t1' t2 t2',
               Si |-co g1 ~: t1 ~~ t2 ->
               Si |-co g2 ~: t1' ~~ t2' ->
+              Si |-ty TArrow t1 t1' ~: KStar ->
+              Si |-ty TArrow t2 t2' ~: KStar ->
               Si |-co CArrow g1 g2 ~: TArrow t1 t1' ~~ TArrow t2 t2'
-| CKApp : forall Si g1 g2 t1 t1' t2 t2',
+| CKApp : forall Si g1 g2 t1 t1' t2 t2' k,
             Si |-co g1 ~: t1 ~~ t2 ->
             Si |-co g2 ~: t1' ~~ t2' ->
+            Si |-ty TApp t1 t1' ~: k ->
+            Si |-ty TApp t2 t2' ~: k ->
             Si |-co CApp g1 g2 ~: TApp t1 t1' ~~ TApp t2 t2'
 | CKLeft : forall Si g t1 t1' t2 t2',
              Si |-co g ~: TApp t1 t1' ~~ TApp t2 t2' ->
@@ -31,24 +37,18 @@ Inductive co_kind : ctxt -> coercion -> type -> type -> Prop :=
 | CKRight : forall Si g t1 t1' t2 t2',
               Si |-co g ~: TApp t1 t1' ~~ TApp t2 t2' ->
               Si |-co CRight g ~: t1' ~~ t2'
-| CKFun : forall Si g t1 t2 f,
+| CKFun : forall Si g t1 t2 f k,
             Si |-co g ~: t1 ~~ t2 ->
+            Si |-ty TFun f t1 ~: k ->
+            Si |-ty TFun f t2 ~: k ->
             Si |-co CFun f g ~: TFun f t1 ~~ TFun f t2
-| CKAx : forall ax ks f typat rhs axs funs tcs tys,
+| CKAx : forall ax ks f typat rhs axs funs tcs tys k,
            ok_ctxt (funs, axs, tcs) -> 
            binds ax (mkAxiom ks f typat rhs) axs ->
+           (funs,axs,tcs) |-ty TFun f (typat[^tys]) ~: k ->
+           (funs,axs,tcs) |-ty rhs[^tys] ~: k ->
            (funs, axs, tcs)|-co CAx ax tys ~: TFun f (typat [^tys]) ~~ (rhs[^tys])
 where "Si |-co g ~: t1 ~~ t2" := (co_kind Si g t1 t2).
-
-Parameter ok__unique : forall {A} x (v v' : A) E,
-  ok E -> binds x v E -> binds x v' E -> v = v'.
-
-Lemma ty_kind_reg : forall Si t k,
-  Si |-ty t ~: k ->
-  ok_ctxt Si.
-Proof.
-  induction 1; try tauto.
-Qed.
 
 Lemma co_kind_reg : forall Si co t1 t2,
   Si |-co co ~: t1 ~~ t2 ->
@@ -58,13 +58,36 @@ Proof.
   eapply ty_kind_reg. eassumption.
 Qed.
 
+Lemma co_kind_reg_tys : forall Si co t1 t2,
+  Si |-co co ~: t1 ~~ t2 ->
+  (exists k1, Si |-ty t1 ~: k1) /\ (exists k2, Si |-ty t2 ~: k2).
+Proof.
+  induction 1; eauto; try tauto.
+  - inverts IHco_kind. inverts H0. inverts H1. inverts H2. inverts H0. eauto.
+  - inverts IHco_kind. inverts H0. inverts H1. inverts H2. inverts H0. eauto.
+Qed.
+
+Lemma co_kind_reg_t1 : forall Si co t1 t2,
+  Si |-co co ~: t1 ~~ t2 ->
+  exists k, Si |-ty t1 ~: k.
+Proof.
+  intros. apply co_kind_reg_tys in H. tauto.
+Qed.
+
+Lemma co_kind_reg_t2 : forall Si co t1 t2,
+  Si |-co co ~: t1 ~~ t2 ->
+  exists k, Si |-ty t2 ~: k.
+Proof.
+  intros. apply co_kind_reg_tys in H. tauto.
+Qed.
+
 Lemma co_kind_det : forall Si co t1 t2,
   Si|-co co ~: t1 ~~ t2 ->
   forall t3 t4,
   Si|-co co ~: t3 ~~ t4 ->
   t1 = t3 /\ t2 = t4.
 Proof.
-  Ltac co_kind_det :=
+  Ltac prove_co_kind_det :=
     repeat match goal with
       | [ IH : forall _ _, _ |-co ?g ~: _ ~~ _ -> _,
             H : _ |-co ?g ~: _ ~~ _
@@ -76,18 +99,42 @@ Proof.
              | [ H : TArrow _ _ = TArrow _ _ |- _ ] => inverts H
            end.
 
-  induction 1; inversion 1; auto; co_kind_det; auto.
+  induction 1; inversion 1; auto; prove_co_kind_det; auto.
   match goal with
     | [ H1 : binds ?ax (mkAxiom ?ks1 ?f1 ?typat1 ?rhs1) _
       , H2 : binds ?ax (mkAxiom ?ks2 ?f2 ?typat2 ?rhs2) _
         |- TFun ?f1 (?typat1 [^_]) = TFun ?f2 (?typat2 [^_]) /\
            ?rhs1[^_] = ?rhs2[^_] ] =>
-      pose proof (ok__unique ax (mkAxiom ks1 f1 typat1 rhs1)
-                                (mkAxiom ks2 f2 typat2 rhs2) axs) as Hunique
-  end. lapplies Hunique. inverts H11. auto. auto. auto. inverts H. tauto.
+      pose proof (@ok__unique axiom ax (mkAxiom ks1 f1 typat1 rhs1)
+                                       (mkAxiom ks2 f2 typat2 rhs2) axs) as Hunique
+  end. lapplies Hunique. inverts H15. auto. auto. auto. inverts H. tauto.
 Qed.
 
+Ltac remove_dups :=
+  repeat match goal with
+    | [ H : ?foo, Hdup : ?foo |- _ ] => clear Hdup
+  end.
+
+Ltac co_kind_det :=
+  let Hl := fresh in
+  let Hr := fresh in
+  remove_dups;
+  match goal with
+    | [ H1 : ?Si |-co ?g ~: ?t1a ~~ ?t2a,
+        H2 : ?Si |-co ?g ~: ?t1b ~~ ?t2b |- _ ] =>
+      apply co_kind_det with (t1 := t1a) (t2 := t2a) in H2; auto;
+      inversion H2 as [Hl Hr]
+  end.
+
+Ltac gen_subst :=
+  repeat match goal with
+           | [ H : ?lhs = ?rhs |- _ ] => first [is_var lhs |
+                                                is_var rhs; symmetry in H]
+         end;
+  subst.
+
 Unset Transparent Obligations.
+Unset Implicit Arguments.
 Program Fixpoint coercionKind funs axs tcs co 
         (_ : exists t1 t2, (funs,axs,tcs)|-co co ~: t1 ~~ t2) 
         { measure (size_of_co false co) } :
@@ -128,28 +175,10 @@ Obligation Tactic :=
   repeat abstract_sig;
   try omega;
   try solve [match goal with
-               | [ H : _ |-co _ ~: _ ~~ _ |- _ ] => inversion H
-             end; simpl; eauto].
+               | [ H : _ |-co _ ~: ?t1 ~~ ?t2 |- _ ] => is_var t1; is_var t2; inversion H
+             end; simpls; repeat co_kind_det; subst; eauto].
 Hint Constructors co_kind.
 Solve Obligations.
-
-Next Obligation.
-  (* trans result *)
-  simpl. eapply CKTrans. simpl in H4. apply H4. simpl in H4.
-  inverts H1.
-  apply co_kind_det with (t1 := H) (t2 := t2) in H4; auto.
-  apply co_kind_det with (t1 := t2) (t2 := H0) in H5; auto.
-  intuition. subst. auto.
-Qed.
-
-Next Obligation.
-  (* arrow result *)
-  simpl. eauto.
-Qed.
-
-Next Obligation.
-  simpl. eauto.
-Qed.
 
 Ltac cant_happen :=
   exfalso; inv_exists;
@@ -186,9 +215,10 @@ Qed.
 
 Next Obligation.
   (* ax result *)
-  inversion H1.
-  subst. econstructor; auto. pose proof H10 as Hcopy. apply binds_get in Hcopy.
-  rewrite Hcopy in Heq_anonymous. inverts Heq_anonymous. eassumption.
+  inverts H1.
+  pose proof H10 as Hcopy. apply binds_get in H10. rewrite H10 in Heq_anonymous.
+  inverts Heq_anonymous.
+  econstructor; eauto.
 Qed.
 
 Next Obligation.
