coercion.v
@@ -19,7 +19,7 @@ Inductive axiom :=
 
 Fixpoint size_of_co (fl : bool) co :=
   match co with
-    | CRefl ty => S (size_of_ty fl ty)
+    | CRefl ty => 0
     | CSym co => S (size_of_co fl co)
     | CTrans co1 co2 => S (size_of_co fl co1 + size_of_co fl co2)
     | CArrow co1 co2 => S (size_of_co fl co1 + size_of_co fl co2)
@@ -27,5 +27,5 @@ Fixpoint size_of_co (fl : bool) co :=
     | CLeft co => S (size_of_co fl co)
     | CRight co => S (size_of_co fl co)
     | CFun _ co => S (size_of_co fl co)
-    | CAx _ tys => S (sum (map (size_of_ty fl) tys))
+    | CAx _ tys => 1
   end.
