ty_kind.v
@@ -1,9 +1,10 @@
 Require Import LibVar.
 Require Import LibEnv.
+Require Import LibTactics.
 
-Require Import type coercion.
+Require Import type coercion var tactics.
 
-Set Implicit Variables.
+Set Implicit Arguments.
 
 Definition fun_ctxt := env (kind * kind).
 Definition ax_ctxt  := env axiom.
@@ -36,3 +37,92 @@ Inductive ty_kind : ctxt -> type -> kind -> Prop :=
             Si |-ty TApp t1 t2 ~: k2
 where "Si |-ty t ~: k" := (ty_kind Si t k).
 
+Lemma ty_kind_reg : forall Si t k,
+  Si |-ty t ~: k -> ok_ctxt Si.
+Proof.
+  induction 1; auto.
+Qed.
+
+Lemma ty_kind_det : forall Si t k1,
+  Si |-ty t ~: k1 ->
+  forall k2,
+  Si |-ty t ~: k2 ->
+  k1 = k2.
+Proof.
+  induction 1; intros.
+  - inverts H1. pose proof (ok__unique f (k1, k2) (k3, k0) funs). lapplies H1.
+    inverts H2. reflexivity.
+    auto. auto. apply ty_kind_reg in H9. unfold ok_ctxt in H9. tauto.
+  - inverts H1. reflexivity.
+  - inverts H1. pose proof (ok__unique T k k2 tcs). lapplies H1.
+    auto. auto. auto. unfolds ok_ctxt. tauto.
+  - inverts H1. apply IHty_kind1 in H5. inverts H5. auto.
+Qed.
+
+Unset Implicit Arguments.
+Program Fixpoint typeKind Si (ty : type) 
+  (Hty : exists k, Si |-ty ty ~: k) :
+  { k : kind | Si |-ty ty ~: k } :=
+  match Si with
+    | (funs, _, tcs) =>
+  match ty with
+    | TBVar _ => _
+    | TFun f ty => match get f funs with
+                     | None => _
+                     | Some (_, kresult) => kresult
+                   end
+    | TArrow arg res => KStar
+    | TTycon T => match get T tcs with
+                    | None => _
+                    | Some k => k
+                  end
+    | TApp t1 _ => let k1 := typeKind Si t1 _ in
+                   match k1 with
+                     | KStar => _
+                     | KArrow _ k2 => k2
+                   end
+  end end.
+
+Next Obligation.
+  exfalso. inverts Hty. inverts H.
+Qed.
+
+Next Obligation.
+  exfalso. inverts Hty. inverts H. apply binds_get in H6. rewrite H6 in Heq_anonymous.
+  discriminate.
+Qed.
+
+Next Obligation.
+  inverts H. pose proof H6.
+  apply binds_get in H6. rewrite H6 in Heq_anonymous. inverts Heq_anonymous. 
+  econstructor; eassumption.
+Qed.
+
+Next Obligation.
+  inverts H. constructor; auto.
+Qed.
+
+Next Obligation.
+  exfalso. inverts Hty. inverts H. apply binds_get in H6. rewrite H6 in Heq_anonymous.
+  discriminate.
+Qed.
+
+Next Obligation.
+  inverts H. pose proof H6.
+  apply binds_get in H6. rewrite H6 in Heq_anonymous. inverts Heq_anonymous.
+  econstructor; eassumption.
+Qed.
+
+Next Obligation.
+  inverts H. eauto.
+Qed.
+
+Next Obligation.
+  exfalso. inverts Hty. inverts H. apply ty_kind_det with (k1 := KStar) in H3; auto.
+  discriminate.
+Defined.
+
+Next Obligation.
+  econstructor. eassumption. inverts H.
+  apply ty_kind_det with (k1 := KArrow k1 Hty) in t; auto. inverts t. auto.
+Defined.
