var.v
@@ -1,5 +1,9 @@
 Require Import LibVar.
+Require Import LibEnv.
 
 Require Import utils.
 
 Axiom var_eq_decide : forall (v1 v2 : var), decide (v1 = v2).
+
+Parameter ok__unique : forall {A} x (v v' : A) E,
+  ok E -> binds x v E -> binds x v' E -> v = v'.
